examples/WellScopedProof/test_indp.v
@@ -64,3 +64,10 @@ with Config : Type :=
   .
 MetaCoq Run Derive InductivePrinciple Point as "indp_point".
 Print indp_point.
+
+
+Inductive myterm2 (A B:Type) : Type :=
+  | myvar : nat -> myterm2 A B
+  | mylam : (nat -> myterm2 A B) -> myterm2 A B.
+MetaCoq Run Derive InductivePrinciple myterm2 as "indp_myterm2".
+Print indp_myterm2.
